\section{Boring proofs}
\label{appendix:boring-proofs}

\subsection*{Complete proof for \reflemma{lemma:indset-sat-graph-td}}

Recall that the depth of the three different components of the elimination forest depicted \reffigure{fig:indset-elimination-forest} are: $tp$ for the trunk, $(p+1)\binom{p}{p/2}$ for the $Clique_i$, and $\O(\log(t\binom{p}{p/2}))$ for the clause gadgets $C_j$. The total treedepth of $G$ is:
\begin{align*}
    \td(G) &\leq tp + (p+1)\binom{p}{p/2} + \O(\log(t\binom{p}{p/2}))\\
    &= tp + \O(\log(t)) + f_1(p) & \text{for some function $f_1$}\\
    &= tp + O(\log \left\lceil\frac{n}{\left\lfloor\log\binom{p}{p/2}\right\rfloor}\right\rceil) + f_1(p) & \text{by definition of $t$}\\
    &= tp + O(\log n) - \O(\log\binom{p}{p/2}) + f_1(p) & \text{$\lfloor\cdot\rfloor$ and $\lceil\cdot\rceil$ disappear in $\O$}\\
    &= tp + O(\log n) + f(p) & \text{for some function $f$}
\end{align*}
which concludes the proof.

\subsection*{Complete proof for \reftheorem{theorem:indset-td-lowerbound}}

Recall Stirling formula: $p! \approx \sqrt{2\pi p}\left(\frac{p}{e}\right)^p$. Thus, we have $\binom{p}{p/2} = \frac{p!}{(p/2)!(p/2)!}\approx \frac{\sqrt{2}}{\sqrt{\pi}}\cdot\frac{2^p}{\sqrt{p}}$.

We have defined $\lambda > 0$ such that $(2-\varepsilon)^{1 + \lambda} \leq (2 - \frac{\varepsilon}{2})$ and $p \geq 2$ such that $p/(p - \frac{1}{2} + \frac{1}{2}\log(\pi p)) \leq 1 + \lambda$. We want to show that $\O^\star((2-\varepsilon)^\td) \leq \O^\star((2-\frac{\varepsilon}{2})^n)$:

\begin{align*}
    \O^\star((2-\varepsilon)^\td) &\leq \O^\star((2-\varepsilon)^{tp + \O(\log n) + f(p)})\\
    &= \O^\star((2-\varepsilon)^{tp}) & \text{since $O^\star$ removes polynomial factors and $f(p)$ is a constant}\\
    &= \O^\star((2-\varepsilon)^{\left(\left\lceil\frac{n}{\left\lfloor\log\binom{p}{p/2}\right\rfloor}\right\rceil\right) p}) & \text{by definition of $t$}\\
    &\approx \O^\star((2-\varepsilon)^{\left(\left\lceil\frac{n}{\left\lfloor\log(\frac{\sqrt{2}}{\sqrt{\pi}}\cdot\frac{2^p}{\sqrt{p}})\right\rfloor}\right\rceil\right) p}) & \text{by Stirling formula}\\
    &\leq \O^\star((2-\varepsilon)^{\left(\frac{n}{\log(\frac{\sqrt{2}}{\sqrt{\pi}}\cdot\frac{2^p}{\sqrt{p}}) - 1} + 1\right)p}) & \text{removing the $\lceil\cdot\rceil$ and $\lfloor\cdot\rfloor$}\\
    &= \O^\star((2-\varepsilon)^{\frac{n}{\frac{1}{2} - \frac{1}{2}\log(\pi p) + p - 1} p + p})\\
    &\leq \O^\star((2-\varepsilon)^{n(1+\lambda) + p}) & \text{by choice of $p$}\\
    &\leq \O^\star((2-\frac{\varepsilon}{2})^{n}) & \text{by definition of $\lambda$}
\end{align*}

which concludes the proof.